riscV/Conventions1.v
@@ -71,8 +71,7 @@ Definition float_callee_save_regs :=
 Definition destroyed_at_call :=
   List.filter (fun r => negb (is_callee_save r)) all_mregs.
 
-Definition dummy_int_reg   := R6.    (**r Used in [Coloring]. *)
-Definition dummy_float_reg := F0 .   (**r Used in [Coloring]. *)
+Definition dummy_regs := R6 :: F0 :: nil. (**r Used in [Coloring]. *)
 
 Definition callee_save_type := mreg_type.
   
@@ -94,17 +93,13 @@ Definition is_float_reg (r: mreg) :=
     only when no caller-save is available. *)
 
 Record alloc_regs := mk_alloc_regs {
-  preferred_int_regs: list mreg;
-  remaining_int_regs: list mreg;
-  preferred_float_regs: list mreg;
-  remaining_float_regs: list mreg
+  preferred_regs: list (list mreg);
+  remaining_regs: list (list mreg)
 }.
 
 Definition allocatable_registers (_: unit) :=
-  {| preferred_int_regs := int_caller_save_regs;
-     remaining_int_regs := int_callee_save_regs;
-     preferred_float_regs := float_caller_save_regs;
-     remaining_float_regs := float_callee_save_regs |}.
+  {| preferred_regs := int_caller_save_regs :: float_caller_save_regs :: nil :: nil;
+     remaining_regs := int_callee_save_regs :: float_callee_save_regs :: nil :: nil|}.
 
 (** * Function calling conventions *)
 
@@ -137,17 +132,18 @@ Definition loc_result (s: signature) : rpair mreg :=
   match proj_sig_res s with
   | Tint | Tany32 => One R10
   | Tfloat | Tsingle | Tany64 => One F10
-  | Tlong => if Archi.ptr64 then One R10 else Twolong R11 R10
+  | Tlong => if Archi.ptr64 then One R10 else Two R11 R10
   end.
 
 (** The result registers have types compatible with that given in the signature. *)
 
 Lemma loc_result_type:
   forall sig,
-  subtype (proj_sig_res sig) (typ_rpair mreg_type (loc_result sig)) = true.
+  subtype (proj_sig_res sig) (mreg_pair_type (loc_result sig)) = true.
 Proof.
   intros. unfold loc_result, mreg_type;
-  destruct (proj_sig_res sig); auto; destruct Archi.ptr64; auto.
+  destruct (proj_sig_res sig); simpl; auto; destruct Archi.ptr64 eqn:E; auto.
+  simpl. destruct Archi.ptr64 eqn:E'; auto.
 Qed.
 
 (** The result locations are caller-save registers *)
@@ -166,7 +162,7 @@ Lemma loc_result_pair:
   forall sg,
   match loc_result sg with
   | One _ => True
-  | Twolong r1 r2 =>
+  | Two r1 r2 =>
        r1 <> r2 /\ proj_sig_res sg = Tlong
     /\ subtype Tint (mreg_type r1) = true /\ subtype Tint (mreg_type r2) = true 
     /\ Archi.ptr64 = false
@@ -275,12 +271,12 @@ Definition split_long_arg (va: bool) (ri rf ofs: Z)
   let ri := if va then align ri 2 else ri in
   match list_nth_z int_param_regs ri, list_nth_z int_param_regs (ri + 1) with
   | Some r1, Some r2 =>
-      Twolong (R r2) (R r1) :: rec (ri + 2) rf ofs
+      Two (R r2) (R r1) :: rec (ri + 2) rf ofs
   | Some r1, None =>
-      Twolong (S Outgoing ofs Tint) (R r1) :: rec (ri + 1) rf (ofs + 1)
+      Two (S Outgoing ofs Tint) (R r1) :: rec (ri + 1) rf (ofs + 1)
   | None, _ =>
       let ofs := align ofs 2 in
-      Twolong (S Outgoing (ofs + 1) Tint) (S Outgoing ofs Tint) ::
+      Two (S Outgoing (ofs + 1) Tint) (S Outgoing ofs Tint) ::
       rec ri rf (ofs + 2)
   end.
 
